extraction/examples/ElmForms.v
@@ -1,0 +1,304 @@
+(** * Elm web app example **)
+
+(** We implement a simple web application allowing for adding users to
+a list after validating the input data. We use the Coq version of
+refinement types (a type with a predicate) to express the fact that
+the list of users contains only valid data. *)
+
+From ConCert.Embedding Require Import CustomTactics.
+From ConCert.Extraction Require Import Common.
+From ConCert.Extraction Require Import Extraction.
+From ConCert.Extraction Require Import ElmExtract.
+From ConCert.Extraction Require Import ElmExtractTests.
+From ConCert.Extraction Require Import Optimize.
+From ConCert.Extraction Require Import Inlining.
+From ConCert.Extraction Require Import PrettyPrinterMonad.
+From ConCert.Extraction Require Import ResultMonad.
+From ConCert.Utils Require Import StringExtra.
+From ConCert.Utils Require Import RecordUpdate.
+
+From Coq Require Import String.
+From Coq Require Import List.
+From Coq Require Import Arith.
+From Coq Require Import Lia.
+From Coq Require Import ssreflect ssrbool.
+From Coq Require Import Program.Program.
+
+From MetaCoq.Template Require Import Ast.
+From MetaCoq.Template Require Import Kernames.
+From MetaCoq.Template Require Import Loader.
+From MetaCoq.Template Require Import TemplateMonad.
+From MetaCoq Require Import monad_utils.
+From MetaCoq Require Import utils.
+
+Open Scope string.
+
+Inductive Cmd (A : Type) : Set :=
+  none.
+
+Arguments none {_}.
+
+(** An entry that corresponds to the user input.
+    Contains "raw" data, potentially invalid *)
+Record Entry :=
+  { name : string;
+    password : string;
+    passwordAgain : string }.
+
+Definition validPassword (p : string) : Prop :=
+  8 <=? String.length p.
+
+Definition nonEmptyString (s : string) : Prop :=
+  s <> "".
+
+(** An entry after validation *)
+Definition ValidEntry :=
+  {entry : Entry | nonEmptyString entry.(name)
+                   /\ validPassword entry.(password)
+                   /\ entry.(password) =? entry.(passwordAgain)}.
+
+
+(** An entry with "raw "data we store in list of users *)
+Record StoredEntry :=
+  { seName : string;
+    sePassword : string }.
+
+(** A valid entry that is stored in the list of users *)
+Definition ValidStoredEntry :=
+  { entry : StoredEntry | nonEmptyString entry.(seName)
+                          /\ validPassword entry.(sePassword)}.
+
+Definition seNames (l : list ValidStoredEntry) :=
+  map (fun x => (proj1_sig x).(seName)) l.
+
+(** The application model *)
+Record Model :=
+  { (** A list of valid entries such with unique user names *)
+    users : {l : list ValidStoredEntry | NoDup (seNames l)};
+    (** A list of erros after validation *)
+    errors : list string;
+    (** Current user input *)
+    currentEntry : Entry }.
+
+
+(** We derive setters for the records in order to use conveninet record update syntax *)
+MetaCoq Run (make_setters Entry).
+MetaCoq Run (make_setters StoredEntry).
+MetaCoq Run (make_setters Model).
+
+(** Messages for updating the model according to the current user input *)
+Inductive Msg :=
+  | MsgName (_ : string)
+  | MsgPassword (_ : string)
+  | MsgPasswordAgain (_ : string).
+
+Definition updateEntry : Msg -> Entry -> Entry :=
+  fun msg model =>
+  match msg with
+    | MsgName newName =>
+       model<| name := newName |>
+    | MsgPassword newPassword =>
+      model<| password := newPassword |>
+    | MsgPasswordAgain newPassword =>
+      model<| passwordAgain := newPassword |>
+  end.
+
+Definition emptyNameError := "Empty name!".
+Definition passwordsDoNotMatchError := "Passwords do not match!".
+Definition passwordIsTooShortError := "Password is too short!".
+Definition userAlreadyExistsError := "User already exists!".
+
+Program Definition validateModel : Model -> list string
+  := fun model =>
+       let res :=
+           [ (~~ existsb (fun nm => nm =? model.(currentEntry).(name)) (seNames model.(users)), userAlreadyExistsError)
+           ; (~~ (model.(currentEntry).(name) =? ""), emptyNameError)
+           ; (model.(currentEntry).(password) =? model.(currentEntry).(passwordAgain), passwordsDoNotMatchError)
+           ; (8 <=? String.length model.(currentEntry).(password), passwordIsTooShortError)] in
+       map snd (filter (fun x => ~~ x.1) res).
+
+
+Inductive StorageMsg :=
+   Add
+ | UpdateEntry (_ : Msg).
+
+
+(** We translate the user input to the stored representation.
+Note that the transation only works for valid entries *)
+Program Definition toStoredEntry : ValidEntry -> StoredEntry
+  := fun entry =>
+       {| seName := entry.(name); sePassword := entry.(password) |}.
+
+Hint Resolve -> eqb_neq : core.
+Hint Unfold nonEmptyString : core.
+
+(** This tactic notation allows to extract information from the fact
+that the validation succeeded *)
+Tactic Notation "destruct_validation" :=
+  unfold validateModel in *;
+  destruct (existsb _ _) eqn:Hexists;
+  destruct (name _ =? "")
+           eqn:name_empty;
+  destruct (password _ =? passwordAgain _)
+           eqn: passwords_eq;
+  destruct (8 <=? String.length (password _))
+           eqn:password_long_enough;tryfalse.
+
+Program Definition updateModel : StorageMsg -> Model -> Model * Cmd StorageMsg
+  := fun msg model =>
+       match msg with
+       | Add =>
+         match validateModel model with
+         | [] => let newEntry : ValidStoredEntry :=
+                    toStoredEntry model.(currentEntry) in
+                 let newList := newEntry :: model.(users) in
+                (model<| users := newList |>, none)
+         | errs => (model<| errors := errs |>, none)
+         end
+       | UpdateEntry entryMsg =>
+         (model<|currentEntry := updateEntry entryMsg model.(currentEntry) |>, none)
+       end.
+Solve Obligations with (cbn;intros;destruct_validation;auto).
+Next Obligation.
+  destruct_validation;auto.
+  constructor.
+  + intro Hin.
+    remember (fun nm : string => nm =? name (currentEntry model)) as f.
+    remember (seNames (proj1_sig model.(users))) as l.
+    assert (Hex_in : exists x, In x l /\ f x = true).
+    { exists model.(currentEntry).(name);subst;split. apply Hin. apply eqb_refl. }
+    now apply existsb_exists in Hex_in.
+  + destruct (model.(users)) as (l, l_nodup). cbn. auto.
+Qed.
+
+Hint Constructors NoDup : core.
+
+Program Definition initModel : Model * Cmd StorageMsg :=
+  let entry :=
+      {| users := []
+       ; errors := []
+       ; currentEntry := Build_Entry "" "" "" |} in
+  (entry, none).
+
+Definition extract_elm_within_coq (should_inline : kername -> bool) :=
+{|
+check_wf_env_func := fun Σ : PCUICAst.PCUICEnvironment.global_env =>
+                     Ok (assume_env_wellformed Σ);
+pcuic_args := {|
+              optimize_prop_discr := true;
+              transforms := [dearg_transform true true true true true
+                            ;Inlining.transform should_inline] |} |}.
+
+Instance ElmBoxes : ElmPrintConfig :=
+  {| term_box_symbol := "()"; (* the inhabitant of the unit type *)
+     type_box_symbol := "()"; (* unit type *)
+     any_type_symbol := "()"; (* unit type *)
+     print_full_names := false |}.
+
+Definition general_wrapped (Σ : global_env) (pre post : string)
+           (seeds : KernameSet.t)
+           (should_inline : list kername)
+           (ignore: list kername) (TT : list (kername * string)) : result string string :=
+  Σ <- extract_template_env
+        (extract_elm_within_coq (fun kn => existsb (eq_kername kn) should_inline))
+         Σ
+         seeds
+         (fun k => existsb (eq_kername k) ignore);;
+  let TT_fun kn := option_map snd (List.find (fun '(kn',v) => eq_kername kn kn') TT) in
+  '(_, s) <- finish_print (print_env Σ TT_fun);;
+  ret (pre ++ nl ++ s ++ nl ++ post).
+
+Record ElmMod :=
+  { elmmd_extract : list ({T : Type & T})}.
+
+Definition USER_FORM_APP : ElmMod :=
+  {| elmmd_extract := [ existT _  updateModel; existT _ initModel] |}.
+
+Definition header_and_imports : string :=
+<$ "module Main exposing (main)"
+; ""
+; "import Browser"
+; "import Html exposing (..)"
+; "import Html.Attributes exposing (..)"
+; "import Html.Events exposing (onInput, onClick)"
+$>.
+
+Definition preamble : string :=
+  <$ "type alias Prod_ a b = (a,b)"
+   ; ""
+   ; "string_eq : String -> String -> Bool"
+   ; "string_eq s1 s2 = s1 == s2"
+   ; ""
+   ; "succ : Int -> Int"
+   ; "succ n = n + 1"
+   ; ""
+   ; "nat_le : Int -> Int -> Bool"
+   ; "nat_le n1 n2 = n1 <= n2"
+   ; ""
+  $>.
+
+Notation "'remap_ctor' c1 'of' ind 'to' c2" := ((<%% ind %%>.1, c1), c2) (at level 100).
+
+  Notation "'string_literal' s" :=
+    (remap <%% s %%> (String.concat "" [""""; s; """"])) (at level 20).
+
+Definition TT :=
+  [ remap <%% bool %%> "Bool"
+  ; remap <%% negb %%> "not"
+
+  ; remap <%% string %%> "String"
+  ; remap <%% String.eqb %%> "string_eq"
+  ; remap <%% String.length %%> "String.length"
+  ; remap_ctor "EmptyString" of string to """"""
+  ; string_literal emptyNameError
+  ; string_literal passwordsDoNotMatchError
+  ; string_literal passwordIsTooShortError
+  ; string_literal userAlreadyExistsError
+
+  ; remap <%% nat %%> "Int"
+  ; remap_ctor "O" of nat to "0"
+  ; remap_ctor "S" of nat to "succ"
+  ; remap <%% Nat.leb %%> "nat_le"
+
+  ; remap <%% prod %%> "Prod_"
+  ; remap_ctor "pair" of prod to "Tuple.pair"
+  ; remap <%% @fst %%> "Tuple.first"
+  ; remap <%% @snd %%> "Tuple.second"
+
+  ; remap <%% list %%> "List"
+  ; remap_ctor "nil" of list to "[]"
+  ; remap_ctor "cons" of list to "(::)"
+  ; remap <%% filter %%> "List.filter"
+  ; remap <%% map %%> "List.map"
+
+  (* Elm infrastructure*)
+  ; remap <%% Cmd %%> "Cmd"
+  ; remap_ctor "none" of Cmd to "Cmd.none"
+  ].
+
+Definition to_inline :=
+  [<%% @setter_from_getter_Entry_name %%>
+  ;<%% setter_from_getter_Model_users %%>
+  ;<%%setter_from_getter_Model_errors %%>
+  ;<%%setter_from_getter_Model_currentEntry%%>
+  ;<%%setter_from_getter_Entry_password%%>
+  ;<%%setter_from_getter_Entry_passwordAgain%%>
+  ].
+
+Definition elm_extraction (m : ElmMod) (TT : list (kername * string)) : TemplateMonad _ :=
+  '(Σ,_) <- tmQuoteRecTransp m false ;;
+  seeds <- monad_map extract_def_name_exists m.(elmmd_extract);;
+  res <- tmEval lazy
+               (general_wrapped
+                  Σ
+                  (header_and_imports ++ nl ++ nl ++ preamble) ""
+                  (KernameSetProp.of_list seeds)
+                  to_inline
+                  (<%% @SetterFromGetter %%> :: map fst TT)
+                  TT);;
+  match res with
+  | Ok prog => tmMsg prog
+  | Err e => tmFail e
+  end.
+
+Redirect "examples/elm-web-extract/UserList.elm" MetaCoq Run (elm_extraction USER_FORM_APP TT).
